Correctness proof for the closure conversion relation. There is an admitted subcase (application of the “observer” function) that requires some discussion about the design of L6 and probably some changes to the semantics.

certicoq/theories/L6_PCPS/closure_conversion_correct.v
@@ -42,7 +42,8 @@ Definition Fun_inv k (rho rho' : env) Scope Funs Γ : Prop :=
         cc_approx_val k (Vfun rho1 B1 f1)
                       (Vconstr tau' t' [(Vfun rho2 B2 f2) ; (Vconstr tau t vs)]).
 
-Lemma Fun_inv_extend k rho rho' Scope Funs Γ
+(* XXX : deprecated *)
+Lemma Fun_inv_extend' k rho rho' Scope Funs Γ
       f rho1 B1 f1 rho2 B2 f2 tau t vs:
   Fun_inv k rho (M.set Γ (Vconstr tau t vs) rho') Scope Funs Γ ->
   f <> Γ ->
@@ -71,6 +72,34 @@ Proof.
       destruct (Coqlib.peq f' Γ); subst.
       * inv Hget2.
       * do 2 (rewrite M.gso; eauto).
+Qed.
+
+Lemma Fun_inv_extend k rho rho' Scope Funs Γ
+      f rho1 B1 f1 rho2 B2 f2 tau t vs:
+  Fun_inv k rho rho' Scope Funs Γ ->
+  f <> Γ ->
+  M.get Γ rho' = Some (Vconstr tau t vs) ->
+  (exists tau' t',
+     cc_approx_val k (Vfun rho1 B1 f1)
+                   (Vconstr tau' t' [(Vfun rho2 B2 f2) ; (Vconstr tau t vs)])) ->
+  Fun_inv k (M.set f (Vfun rho1 B1 f1) rho)
+          (M.set f  (Vfun rho2 B2 f2) rho')
+          Scope (Union _ (Singleton _ f) Funs) Γ.
+Proof.
+  intros Hinv Hneq Hget Hv. edestruct Hinv as [tau' [t' [vs' [Hget' Hyp]]]].
+  do 3 eexists. rewrite M.gso; eauto. split; [ eassumption |].
+  intros f' v Hnin Hin Hget''. rewrite Hget in Hget'. inv Hget'.
+  rewrite M.gsspec in Hget''. destruct (Coqlib.peq f' f); subst.
+  - inv Hget''.
+    edestruct Hv as [tau1 [t1 Happrox]]; eauto.
+    repeat eexists. rewrite M.gss; eauto.
+    eassumption.
+  - edestruct Hyp as
+        [rho3 [B3 [f3 [rho4 [B4 [f4 [tau2 [t2 [Heq [Hget2 Happrox]]]]]]]]]];
+    subst; eauto.
+    + inv Hin; eauto. inv H. congruence.
+    + repeat eexists; eauto.
+      rewrite M.gso; eauto.
 Qed.
 
 Lemma closure_conversion_fundefs_find_def Funs FVs B1 B2 f t1 xs e1 :
@@ -240,6 +269,155 @@ Proof.
       eapply Included_Union_r.
 Qed.
 
+Lemma Closure_conversion_fundefs_name_in_fundefs Funs FVs B1 B2  :
+  Closure_conversion_fundefs Funs FVs B1 B2 ->
+  Same_set _ (name_in_fundefs B1) (name_in_fundefs B2).
+Proof.
+  intros Hcc. induction Hcc; simpl.
+  - eapply Same_set_Union_compat.
+    now eapply Same_set_refl.
+    now eauto.
+  - now apply Same_set_refl.
+Qed.
+
+Lemma Fun_inv_reset k rho rho' B v Scope Funs Γ :
+  ~ In _ (name_in_fundefs B) Γ ->
+  Fun_inv k rho
+          (def_funs B B (M.set Γ v rho') (M.set Γ v rho')) Scope Funs Γ ->
+  Fun_inv k rho
+          (M.set Γ v (def_funs B B (M.set Γ v rho') (M.set Γ v rho')))
+          Scope Funs Γ.
+Proof. 
+  intros Hin [tau [t [vs [Hget Hfun]]]]. 
+  rewrite def_funs_neq in Hget; eauto. rewrite M.gss in Hget.
+  inv Hget.
+  do 3 eexists. rewrite M.gss. split; eauto.
+  intros f v Hnin Hin' Hget.
+  edestruct Hfun as
+      [rhof1 [B1 [f1 [rhof2 [B2 [f2 [tau' [t' [Heq [Hget' Hcc]]]]]]]]]]; eauto.
+  subst. eapply def_funs_spec in Hget'.
+  destruct Hget' as [[Hname Heq] | [Hname Hget']].
+  - inv Heq. repeat eexists; eauto.
+    rewrite M.gso.
+    rewrite def_funs_eq. reflexivity. eassumption.
+    intros Hc; subst; eauto.
+  - rewrite M.gsspec in Hget'.
+    destruct (Coqlib.peq f Γ).
+    + subst. inv Hget'.
+    + repeat eexists; eauto. rewrite M.gso. 
+      rewrite def_funs_neq; eauto. 
+      rewrite M.gso. eassumption.
+      intros Hc; subst; eauto.
+      intros Hc; subst; eauto.
+Qed.
+
+Lemma get_def_funs_In_names B' B f rho :
+  In var (name_in_fundefs B) f ->
+  exists v : val, M.get f (def_funs B' B rho rho) = Some v.
+Proof.
+  induction B; intros Hin; inv Hin. 
+  - inv H. eexists. simpl. rewrite M.gss. eauto.
+  - edestruct IHB as [v' Heq]; eauto.
+    destruct (Coqlib.peq f v) eqn:Heq'.
+    + eexists. simpl. now rewrite M.gsspec, Heq'.
+    + eexists. simpl. rewrite M.gsspec, Heq'.
+      eassumption.
+Qed.
+
+Lemma get_setlist_In_xs x xs vs rho rho' :
+  In var (FromList xs) x ->
+  setlist xs vs rho = Some rho' ->
+  exists v : val, M.get x rho' = Some v.
+Proof.
+  revert rho rho' vs. induction xs; intros rho rho' vs Hin Hset.
+  - rewrite FromList_nil in Hin. exfalso.
+    eapply not_In_Empty_set. eassumption. 
+  - rewrite FromList_cons in Hin.
+    destruct vs; try discriminate.    
+    simpl in Hset. destruct (setlist xs vs rho) eqn:Hsetlist; try discriminate.
+    inv Hset. inv Hin.
+    + inv H. eexists. rewrite M.gss. reflexivity.
+    + destruct (Coqlib.peq x a); subst.
+      * eexists. now rewrite M.gss.
+      * edestruct IHxs; eauto.
+        eexists. simpl. rewrite M.gso; eauto. 
+Qed.
+
+Definition vars_in_env S (rho : env) : Prop :=
+  forall x, In _ S x -> exists v, M.get x rho = Some v. 
+
+Inductive unique_functions : fundefs -> Prop :=
+| Fnil_un :
+    unique_functions Fnil
+| Fcons_un :
+    forall f tau xs e B,
+      unique_functions B ->
+      ~ In _ (name_in_fundefs B) f ->
+      unique_functions (Fcons f tau xs e B).
+
+Definition fundefs_names_unique (e : exp) : Prop :=
+  forall B, funs_in_exp B e -> unique_functions B.
+
+Definition fundefs_names_unique_fundefs (B : fundefs) : Prop :=
+  forall B', funs_in_fundef B' B \/ B' = B -> unique_functions B'.
+
+Lemma vars_in_env_antimon S S' rho :
+  Included _ S' S ->
+  vars_in_env S rho ->
+  vars_in_env S' rho.
+Proof.
+  intros Hin Hv x Hs. eauto.
+
+Qed.
+
+Lemma vars_in_env_extend x v S rho :
+  vars_in_env S rho ->
+  vars_in_env (Union _ S (Singleton _ x)) (M.set x v rho).
+Proof. 
+  intros H x' Hs. inv Hs.
+  - edestruct H; eauto.
+    destruct (Coqlib.peq x' x) eqn:Heq'.
+    + eexists. simpl. now rewrite M.gsspec, Heq'.
+    + eexists. simpl. rewrite M.gsspec, Heq'.
+      eassumption.
+  - inv H0. eexists. rewrite M.gss. eauto.
+Qed.
+
+Instance Decidable_FromList (l : list var) : Decidable (FromList l). 
+Proof. 
+  constructor. intros x. induction l. 
+  - right. intros H. inv H. 
+  - destruct (Coqlib.peq a x).
+    + subst. left. constructor. eauto.
+    + destruct IHl. left. now constructor 2.
+      right. intros Hc. eapply H. inv Hc; eauto.
+      congruence.
+Qed.
+
+Lemma vars_in_env_setlist xs vs S rho rho' :
+  vars_in_env S rho ->
+  setlist xs vs rho = Some rho' ->
+  vars_in_env (Union _ (FromList xs) S) rho'.
+Proof.
+  intros H Hset x' Hs.
+  destruct (Decidable_FromList xs). destruct (Dec x').
+  - eapply get_setlist_In_xs; eauto.
+  - destruct Hs; try contradiction. 
+    edestruct H; eauto.
+    eexists. erewrite <- setlist_not_In; eauto.
+Qed.
+
+Lemma vars_in_env_def_funs B' B rho S  :
+  vars_in_env S rho ->
+  vars_in_env (Union _ (name_in_fundefs B) S) (def_funs B' B rho rho).
+Proof.
+  intros H x' Hs.
+  destruct (Decidable_name_in_fundefs B). destruct (Dec x').
+  - eapply get_def_funs_In_names; eauto.
+  - destruct Hs; try contradiction. 
+    edestruct H; eauto.
+    eexists. erewrite def_funs_neq; eauto.
+Qed.
 
 Lemma closure_conversion_fundefs_correct k rho rho' B1 B2 B1' B2'
       Scope Γ FVs Funs' FVs' t tau vs:
@@ -250,53 +428,71 @@ Lemma closure_conversion_fundefs_correct k rho rho' B1 B2 B1' B2'
        (Scope Funs : Ensemble var) (Γ : var) (FVs : list M.elt),
        cc_approx_env_P Scope m rho rho' ->
        ~ In var (bound_var e) Γ ->
+       vars_in_env (occurs_free e) rho ->
+       fundefs_names_unique e ->
        Fun_inv m rho rho' Scope Funs Γ ->
        env_inv m rho rho' Scope Funs Γ FVs ->
        Closure_conversion Scope Funs Γ FVs e e' ->
        cc_approx_exp m (e, rho) (e', rho')) ->
   Same_set _ (occurs_free_fundefs B1) (FromList FVs) ->
+  fundefs_names_unique_fundefs B1 ->
+  vars_in_env (occurs_free_fundefs B1) rho ->
   Closure_conversion_fundefs (name_in_fundefs B1) FVs B1 B2 ->
   Closure_conversion_fundefs Funs' FVs' B1' B2' ->
   ~ In _ (name_in_fundefs B1) Γ ->
   ~ In _ (name_in_fundefs B1') Γ ->
   closure_env k rho (Empty_set _) (Empty_set _) vs FVs ->
   Fun_inv k (def_funs B1 B1' rho rho)
-          (M.set Γ (Vconstr tau t vs) (def_funs B2 B2' rho' rho'))
+          (def_funs B2 B2' (M.set Γ (Vconstr tau t vs) rho') (M.set Γ (Vconstr tau t vs) rho'))
           Scope (name_in_fundefs B1') Γ.
 Proof.
   revert B1' rho rho' B2 B1 B2' Scope Γ FVs Funs' FVs' t tau vs.
   induction k as [k IHk] using lt_wf_rec1.
-  induction B1';
+  induction B1'; 
     intros rho rho' B2 B1 B2' Scope Γ FVs Funs' FVs' t' tau' vs
-           IHe Hs Hcc Hcc' Hnin Hnin' Henv.
+           IHe Hs Hun Hfv Hcc Hcc' Hnin Hnin' Henv.
   - inv Hcc'. simpl.
     eapply Fun_inv_extend.
     + eapply IHB1'; eauto.
       intros Hc. apply Hnin'.
       simpl; eauto.
     + intros Hc. apply Hnin'. subst. simpl; eauto.
+    + rewrite def_funs_neq.
+      rewrite M.gss. reflexivity.
+      simpl in Hnin'.
+      rewrite Closure_conversion_fundefs_name_in_fundefs in Hnin';
+        [now eauto | eassumption ].
     + exists tau', t.
       rewrite cc_approx_val_eq.
       intros vs1 vs2 j t1 xs1 e1 rho1' Hlen Hfind Hset.
       edestruct setlist_length
-      with (rho' := def_funs B2 B2 rho' rho') as [rho2' Hset']. eassumption.
-      now eauto.
+      with (rho' := def_funs B2 B2 (M.set Γ (Vconstr tau' t' vs) rho')
+                             (M.set Γ (Vconstr tau' t' vs) rho')) as [rho2' Hset'].
+      eassumption. now eauto.
       edestruct closure_conversion_fundefs_find_def
         as [t2 [Γ'' [e2 [Hnin'' [Hfind' Hcc']]]]]; [| eassumption |]. eassumption.
       exists t2, Γ'', xs1. do 2 eexists.
       split. eassumption. split.
       simpl. rewrite Hset'. reflexivity.
-      intros Hlt Hall. 
-      eapply IHe; try eassumption.
+      intros Hlt Hall.  
+      eapply IHe; try eassumption.  
       * eapply cc_approx_env_P_set_not_in_P_r.
         eapply cc_approx_env_P_setlist_l with (P1 := Empty_set _); eauto. 
         eapply cc_approx_env_Empty_set.
         intros x H1 H2. contradiction.
         constructor. intros x Hc. inv Hc. inv H0. eauto.
       * intros Hc. apply Hnin''. eauto.
+      * eapply vars_in_env_antimon.
+        eapply occurs_free_in_fun. eapply find_def_correct. eassumption.
+        eapply vars_in_env_setlist; [| now eauto ].
+        eapply vars_in_env_def_funs. eassumption.
+      * intros B Hin. eapply Hun. left. 
+        eapply fun_in_fundefs_funs_in_fundef; eauto.
+        eapply find_def_correct. eassumption.
       * assert
           (Fun_inv j (def_funs B1 B1 rho rho)
-                   (M.set Γ (Vconstr tau' t' vs) (def_funs B2 B2 rho' rho'))
+                   (def_funs B2 B2 (M.set Γ (Vconstr tau' t' vs) rho')
+                             (M.set Γ (Vconstr tau' t' vs) rho'))
                    (FromList xs1) (name_in_fundefs B1) Γ).
         { eapply IHk; try eassumption.
           - intros. eapply IHe; eauto. omega. 
@@ -306,8 +502,10 @@ Proof.
             eassumption. omega. } 
         eapply Fun_inv_rename with (Γ := Γ); eauto.
         eapply Fun_inv_setlist_In_Scope_l; [ now apply Included_refl | |].
-        eapply Fun_inv_setlist_In_Scope_r; [ now apply Included_refl | |].
-        eassumption. now eauto. now eauto.
+        eapply Fun_inv_setlist_In_Scope_r; [ now apply Included_refl | |]. 
+        eapply Fun_inv_reset; [| eassumption ].
+        rewrite <- Closure_conversion_fundefs_name_in_fundefs; [ | eassumption ].
+        now eauto. now eauto. now eauto.
       * do 3 eexists. split.
         rewrite M.gss. reflexivity.
         intros x N v1 Hnin1 Hnin2 Hnth Hget'. 
@@ -319,10 +517,10 @@ Proof.
         now eauto. now eauto. now eauto.
         eexists; eauto. split. eassumption.
         eapply cc_approx_val_monotonic. eassumption. omega.
-  - do 3 eexists. rewrite M.gss. split; eauto.
-    intros. inv H0.
+  - do 3 eexists.
+    rewrite def_funs_neq. rewrite M.gss. split; eauto.
+    intros. inv H0. inv Hcc'. simpl. eauto.
 Qed.
-
 
 (* Fixpoint ctx_as_env (rho : env) v C : env := *)
 (*   match C with *)
@@ -372,6 +570,16 @@ Proof.
   rewrite M.gsspec in Hget'. destruct (Coqlib.peq y x); subst.
   - contradiction. 
   - eauto. 
+Qed.
+
+Lemma env_inv_extend_In_Scope_r k rho rho' x v Scope Funs FVs Γ :
+  In var Scope x ->
+  x <> Γ ->
+  env_inv k rho rho' Scope Funs Γ FVs ->
+  env_inv k rho (M.set x v rho') Scope Funs Γ FVs.
+Proof.
+  intros Hin Hneq HInv. destruct HInv as [tau [t  [vs [Hget H]]]].
+  do 3 eexists; split; eauto. rewrite M.gso; eauto.
 Qed.
 
 Lemma nthN_In {A} (l : list A) n v :
@@ -518,6 +726,74 @@ Proof.
       rewrite H11 in Hnth. now inv Hnth.
 Qed.
 
+Lemma project_var_not_In_free_set  Scope Funs Γ FVs x x' C S S'  :
+  project_var Scope Funs Γ FVs S x x' C S' ->
+  Disjoint _ S (Union var Scope
+                      (Union var Funs
+                             (Union var (FromList FVs) (Singleton var Γ)))) ->
+  ~ In _ S' x'.
+Proof.
+  intros Hproj Hd. inv Hproj; intros Hc.
+  - eapply Hd. eauto.
+  - inv Hc. exfalso. eauto.
+  - inv Hc. exfalso. eauto.    
+Qed.
+
+Lemma project_var_free_set_Included Scope Funs Γ FVs x x' C S S' :
+  project_var Scope Funs Γ FVs S x x' C S' ->
+  Included _ S' S.
+Proof.
+  intros Hproj. inv Hproj.
+  - now apply Included_refl.
+  - now apply Subset_Setminus.
+  - now apply Subset_Setminus.
+Qed.
+
+Lemma project_vars_free_set_Included Scope Funs Γ FVs xs xs' C S S' :
+  project_vars Scope Funs Γ FVs S xs xs' C S' ->
+  Included _ S' S.
+Proof.
+  intros Hproj. induction Hproj.
+  - now apply Included_refl.
+  - eapply Included_trans. eassumption.
+    eapply project_var_free_set_Included. eassumption. 
+Qed.
+
+Lemma project_vars_not_In_free_set  Scope Funs Γ FVs xs xs' C S S'  :
+  project_vars Scope Funs Γ FVs S xs xs' C S' ->
+  Disjoint _ S (Union var Scope
+                      (Union var Funs
+                             (Union var (FromList FVs) (Singleton var Γ)))) ->
+  Disjoint _ S' (FromList xs').
+Proof.
+  intros Hproj Hd. induction Hproj.
+  - constructor.  intros x Hc. inv Hc. rewrite FromList_nil in H0.
+    eapply not_In_Empty_set. eassumption. 
+  - rewrite FromList_cons. eapply Disjoint_sym.
+    eapply Disjoint_Union.
+    + eapply Disjoint_sym. eapply Disjoint_Included_l.
+      eapply project_vars_free_set_Included. eassumption.
+      eapply Disjoint_Singleton.
+      eapply project_var_not_In_free_set; eassumption. 
+    + eapply Disjoint_sym. eapply IHHproj.
+      eapply Disjoint_Included_l.
+      eapply project_var_free_set_Included. eassumption.
+      eassumption.
+Qed.
+
+Lemma getlist_set_neq {A} xs x (v : A) rho :
+  ~ List.In x xs ->
+  getlist xs (M.set x v rho) = getlist xs rho. 
+Proof.
+  intros Hin.
+  revert rho. induction xs; intros rho.
+  - reflexivity.
+  - simpl. rewrite M.gso.
+    + rewrite IHxs. reflexivity.
+      intros Hin'. eapply Hin. now constructor 2.
+    + intros Heq; subst. eapply Hin. now constructor.
+Qed.
+
 Lemma ctx_to_rho_comp_ctx C C1 C2 rho rho' :
   ctx_to_rho C rho rho' ->
   comp_ctx C1 C2 C ->
@@ -558,25 +834,6 @@ Proof.
   - simpl; econstructor; eauto.
 Qed.
 
-Lemma project_var_free_set_Included Scope Funs Γ FVs x x' C S S' :
-  project_var Scope Funs Γ FVs S x x' C S' ->
-  Included _ S' S.
-Proof.
-  intros Hproj. inv Hproj.
-  - now apply Included_refl.
-  - now apply Subset_Setminus.
-  - now apply Subset_Setminus.
-Qed.
-
-Lemma project_vars_free_set_Included Scope Funs Γ FVs xs xs' C S S' :
-  project_vars Scope Funs Γ FVs S xs xs' C S' ->
-  Included _ S' S.
-Proof.
-  intros Hproj. induction Hproj.
-  - now apply Included_refl.
-  - eapply Included_trans. eassumption.
-    eapply project_var_free_set_Included. eassumption. 
-Qed.
 
 Lemma project_var_get Scope Funs Γ FVs S1 x x' C1 S2 rho1 rho2 y:
   project_var Scope Funs Γ FVs S1 x x' C1 S2 ->
@@ -894,10 +1151,236 @@ Proof.
   inv Hin'. eauto.
 Qed.
 
-                     
+Lemma make_closures_correct k rho1 rho2 rho2' B Scope Funs FVs Γ Γ' C :
+  make_closures B Γ' C ->
+  unique_functions B ->
+  ~ In _ (name_in_fundefs B) Γ ->
+  ~ In _ (name_in_fundefs B) Γ' ->
+  Included _ (name_in_fundefs B) Scope ->
+  cc_approx_env_P (Setminus _ Scope (name_in_fundefs B)) k rho1 rho2 ->
+  Fun_inv k rho1 rho2 Scope Funs Γ ->  
+  env_inv k rho1 rho2 Scope Funs Γ FVs ->
+  Fun_inv k rho1 rho2 (Empty_set _) (name_in_fundefs B) Γ' ->
+  ctx_to_rho C rho2 rho2' ->
+  cc_approx_env_P Scope k rho1 rho2' /\
+  Fun_inv k rho1 rho2' Scope Funs Γ /\
+  env_inv k rho1 rho2' Scope Funs Γ FVs.
+Proof.
+  intros Hmake. revert k rho1 rho2 rho2' Scope Funs FVs Γ.
+  induction Hmake;
+    intros k rho1 rho2 rho2' Scope Funs FVs Γ1 Hun Hnin1 Hnin2
+           Hsub Hcc Hfun Henv Hfun' Hctx.
+  - inv Hctx. repeat split; eauto.
+    simpl in *.
+    now rewrite Setminus_Empty_set_Same_set in Hcc. 
+  - eapply ctx_to_rho_comp_ctx in Hctx; [| apply Constr_cc; constructor ].
+    destruct Hctx as [rho2'' [Hctx1 Hctx2]].
+    inv Hctx1. inv H9. inv Hun.
+    (* destruct Hfun as [tau1 [t1 [vs [Hget Hfun]]]]. *)
+    edestruct IHHmake as [Hcc1 [Hfun1 Henv1]];
+      [ eassumption | | | | | | | | eassumption | ].
+    + intros Hc. eapply Hnin1. right. now apply Hc. 
+    + intros Hc. eapply Hnin2. right. now apply Hc. 
+    + eapply Included_trans; [| eassumption ].
+      now eapply Included_Union_r.
+    + eapply cc_approx_env_P_antimon;
+      [| now apply (@Included_Union_Setminus _ _ (Singleton var f) _) ].
+      rewrite Setminus_Union, (Union_sym (name_in_fundefs B)).
+      eapply cc_approx_env_P_union.
+      eapply cc_approx_env_P_not_in_P_r. eassumption.
+      intros Hc. inv Hc. now eauto.
+      intros f' Hs v Hget'. inv Hs.
+      edestruct Hfun' as [tau2 [t2 [vs2 [Hget2 Hfun2]]]]. 
+      edestruct Hfun2
+        as [rho1f' [B1 [f1 [rho2f' [B2 [f2 [tau2' [t2' [Heq' [Hget2' Happrox2]]]]]]]]]]; eauto.
+      now eapply not_In_Empty_set. now left; eauto.
+      subst. eexists; split.
+      rewrite M.gss. reflexivity.
+      rewrite H8 in Hget2'. inv Hget2'. rewrite H7 in Hget2. inv Hget2.
+      rewrite cc_approx_val_eq in *. now eauto.
+    + eapply Fun_inv_set_In_Scope_r_not_Γ ; [| | eassumption ].
+      * eapply Hsub. now left. 
+      * intros Hc; subst. eapply Hnin1. left; eauto.
+    + eapply env_inv_extend_r; [| eassumption ].
+      intros Hc; subst. eapply Hnin1. left; eauto.
+    + edestruct Hfun' as [tau2 [t2 [vs2 [Hget2 Hfun2]]]]. 
+      do 3 eexists; split; eauto.
+      rewrite M.gso. eassumption.
+      intros Hc; subst. eapply Hnin2. left; eauto.
+      intros f' v' _ Hnin Hgetf. 
+      edestruct Hfun2
+        as [rho1f' [B1 [f1 [rho2f' [B2 [f2 [tau2' [t2' [Heq' [Hget2' Happrox2]]]]]]]]]]; eauto.
+      now eapply not_In_Empty_set. now right; eauto.
+      repeat eexists; eauto. 
+      rewrite M.gso. eassumption.
+      intros Hc; subst; eauto.
+    + eauto.
+Qed. 
+
+Lemma make_closures_ctx_to_rho B Γ C k rho1 rho2  :
+  make_closures B Γ C ->
+  unique_functions B ->
+  ~ In _ (name_in_fundefs B) Γ ->
+  Fun_inv k rho1 rho2 (Empty_set _) (name_in_fundefs B) Γ ->
+  (forall f, In _ (name_in_fundefs B) f -> exists v, M.get f rho1 = Some v) ->
+  exists rho2', ctx_to_rho C rho2 rho2'.
+Proof. 
+  intros Hclo. revert rho1 rho2. induction Hclo; intros rho1 rho2 Hun Hnin Hfun Hyp. 
+  - eexists; constructor. 
+  - destruct (Hyp f) as [v' Hget'].
+    now left; eauto.
+    edestruct Hfun as [tau1 [t1 [vs1 [Hget1 Hfun']]]].
+    edestruct Hfun' as
+        [rho1f' [B1 [f1 [rho2f' [B2 [f2 [tau2 [t2 [Heq' [Hget2 Happrox2]]]]]]]]]]; eauto.
+    now apply not_In_Empty_set.
+    now left; eauto. inv Hun.
+    edestruct IHHclo as [rho2' Hctx]; [ eassumption | | | | now eexists; econstructor; eauto]. 
+    + intros Hc; eapply Hnin; right; eauto.
+    + eapply Fun_inv_set_not_In_Funs_r_not_Γ; [ eassumption | | ].
+      intros Hc; subst. eapply Hnin; now left. 
+      do 3 eexists; split; eauto; intros.
+      edestruct Hfun' as
+          [rho1'' [B1' [f1' [rho2'' [B2' [f2' [tau2' [t2' [Heq'' [Hget2' Happrox2']]]]]]]]]]; eauto.
+      right; eauto. 
+      subst. repeat eexists; eauto.
+    + intros. eapply Hyp. right; eauto.
+Qed.
+
+Lemma getlist_nth_get (xs : list var) (vs : list val) rho (x : var) N :
+  getlist xs rho = Some vs ->
+  nthN xs N = Some x ->
+  exists v, nthN vs N = Some v /\ M.get x rho = Some v. 
+Proof.
+  revert vs N; induction xs; intros vs N Hget Hnth.
+  - inv Hnth. 
+  - simpl in Hget.
+    destruct (M.get a rho) eqn:Hget'; try discriminate.
+    destruct (getlist xs rho) eqn:Hgetlist'; try discriminate.
+    inv Hget. destruct N. 
+    + inv Hnth. eexists; simpl; eauto.
+    + edestruct IHxs as [v' [Hnth1 Hget1]]; eauto. 
+Qed.
+
+Lemma In_getlist (xs : list var) (rho : env) :
+  (forall x, List.In x xs -> exists v, M.get x rho = Some v) ->
+  exists vs, getlist xs rho = Some vs. 
+Proof.                                            
+  intros H. induction xs. 
+  - eexists; simpl; eauto.
+  - edestruct IHxs. 
+    + intros x Hin. eapply H. now constructor 2. 
+    + edestruct H. now constructor. 
+      eexists. simpl. erewrite H1, H0. 
+      reflexivity. 
+Qed.
+
+Lemma Fun_inv_def_funs_l k rho rho' B1 B1' Scope Funs Γ:
+  Fun_inv k rho rho' Scope Funs Γ ->
+  Fun_inv k (def_funs B1 B1' rho rho) rho'
+          (Union _ (name_in_fundefs B1')  Scope) Funs Γ.
+Proof.
+  intros [t [tau [v [Hget Hfun]]]].
+  do 3 eexists. split; eauto.
+  intros f v' Hnin Hin Hget'.
+  rewrite def_funs_neq in Hget'; eauto.
+Qed.
+
+Lemma Fun_inv_def_funs_r k rho rho' B1 B1' Scope Funs Γ:
+  ~ In _ (name_in_fundefs B1') Γ ->
+  Fun_inv k rho rho' Scope Funs Γ ->
+  Fun_inv k rho (def_funs B1 B1' rho' rho')
+          (Union _ (name_in_fundefs B1') Scope) Funs Γ.
+Proof.
+  intros Hin [t [tau [v [Hget Hfun]]]].
+  do 3 eexists. split; eauto. 
+  rewrite def_funs_neq; eauto.
+  intros f v' Hnin Hin' Hget'.
+  edestruct Hfun as
+      [rho1' [B2 [f1 [rho2' [B2' [f2 [tau2 [t2 [Heq' [Hget2 Happrox2]]]]]]]]]]; eauto.
+  repeat eexists; eauto.
+  rewrite def_funs_neq; eauto.
+Qed.
+
+Instance Fun_inv_proper :
+  Proper (Logic.eq ==> Logic.eq ==> Logic.eq ==> Same_set var ==> Logic.eq ==> Logic.eq ==> iff)
+         (Fun_inv).
+Proof.
+  constructor; subst; intros [tau [t [vs [Hget Hfun]]]]; do 3 eexists; split; eauto;
+  intros; eapply Hfun; eauto; intros Hc; eapply H; eapply H2; eauto.
+Qed.
+
+Lemma Fun_inv_def_funs k rho rho' B1 B1' B2 B2' Scope Funs Γ:
+  ~ In _ (name_in_fundefs B1') Γ ->
+  Same_set _ (name_in_fundefs B1') (name_in_fundefs B2') ->
+  Fun_inv k rho rho' Scope Funs Γ ->
+  Fun_inv k  (def_funs B1 B1' rho rho) (def_funs B2 B2' rho' rho')
+          (Union _ (name_in_fundefs B1') Scope) Funs Γ.
+Proof.
+  intros Hin HS [t [tau [v [Hget Hfun]]]].
+  do 3 eexists. split; eauto. 
+  rewrite def_funs_neq; eauto.
+  intros Hc. eapply Hin. now eapply HS.
+  intros f v' Hnin Hin' Hget'.
+  rewrite def_funs_neq in Hget'; eauto.
+  edestruct Hfun as
+      [rho1' [B3 [f1 [rho2' [B3' [f2 [tau2 [t2 [Heq' [Hget2 Happrox2]]]]]]]]]]; eauto.
+  repeat eexists; eauto.
+  rewrite def_funs_neq; eauto.
+  intros Hc. eapply Hnin. left. now rewrite HS.
+Qed.
+
+Lemma cc_approx_env_P_def_funs_not_In_P_l k rho1 rho2 S B B' :
+  Disjoint _ S (name_in_fundefs B') ->
+  cc_approx_env_P S k rho1 rho2 ->
+  cc_approx_env_P S k (def_funs B B' rho1 rho1) rho2.
+Proof.
+  intros Hd Hcc x HS v Hget. eapply Hcc; eauto. 
+  erewrite <- def_funs_neq. eassumption.  
+  intros Hc. eapply Hd; constructor; eauto.
+Qed.
+
+Lemma cc_approx_env_P_def_funs_not_In_P_r k rho1 rho2 S B B' :
+  Disjoint _ S (name_in_fundefs B') ->
+  cc_approx_env_P S k rho1 rho2 ->
+  cc_approx_env_P S k rho1 (def_funs B B' rho2 rho2).
+Proof.
+  intros Hd Hcc x HS v Hget.
+  edestruct Hcc as [v' [Hget' Hcc']]; eauto.
+  eexists; split; eauto.
+  rewrite def_funs_neq. eassumption.
+  intros Hc. eapply Hd; constructor; eauto.
+Qed.
+
+Lemma env_inv_def_funs k rho rho' B1 B1' B2 B2' Scope Funs Γ FVs:
+  ~ In _ (name_in_fundefs B1') Γ ->
+  Same_set _ (name_in_fundefs B1') (name_in_fundefs B2') ->
+  env_inv k rho rho' Scope Funs Γ FVs ->
+  env_inv k  (def_funs B1 B1' rho rho) (def_funs B2 B2' rho' rho')
+          (Union _ (name_in_fundefs B1') Scope) Funs Γ FVs.
+Proof.
+  intros Hin HS [t [tau [v [Hget Henv]]]].
+  do 3 eexists. split; eauto. 
+  rewrite def_funs_neq; eauto.
+  intros Hc. eapply Hin. now eapply HS.
+  intros f N v' Hnin Hnin' Hnth Hget'.
+  rewrite def_funs_neq in Hget'; eauto.
+Qed.
+
+Corollary Fun_inv_def_funs' k rho rho' B1 B1' B2 B2' Scope Funs Γ:
+  ~ In _ (name_in_fundefs B1') Γ ->
+  Same_set _ (name_in_fundefs B1') (name_in_fundefs B2') ->
+  Fun_inv k rho rho' Scope Funs Γ ->
+  Fun_inv k  (def_funs B1 B1' rho rho) (def_funs B2 B2' rho' rho')
+          (Union _ (name_in_fundefs B2') Scope) Funs Γ.
+Proof.
+  intros Hin HS Hf. rewrite <- HS. now apply Fun_inv_def_funs.
+Qed.
+
 Lemma closure_conversion_correct k rho rho' e e' Scope Funs Γ FVs :
   cc_approx_env_P Scope k rho rho' ->
   ~ In _ (bound_var e) Γ ->
+  vars_in_env (occurs_free e) rho ->
+  fundefs_names_unique e ->
   Fun_inv k rho rho' Scope Funs Γ ->
   env_inv k rho rho' Scope Funs Γ FVs ->
   Closure_conversion Scope Funs Γ FVs e e' ->
@@ -906,8 +1389,8 @@ Proof.
   revert k e rho rho' e' Scope Funs Γ FVs.
   induction k as [k IHk] using lt_wf_rec1.
   induction e using exp_ind';
-    intros rho1 rho2 e' Scope Funs Γ FVs Happrox Hnin Hfun Henv Hcc.
-  - (* Case Econstr. Induction on l and then similar to Eproj *)
+    intros rho1 rho2 e' Scope Funs Γ FVs Happrox Hnin HFVs Hun Hfun Henv Hcc.
+  - (* Case Econstr *)
     inv Hcc.
     intros v1 c1 Hleq Hstep. inv Hstep.
     edestruct project_vars_ctx_to_rho as [rho2' Hto_rho]; eauto.
@@ -917,9 +1400,9 @@ Proof.
     edestruct Hvar as [v' [Hget' Happ']]; eauto.
     eapply ctx_to_rho_cc_approx_exp; eauto.
     intros v1' c1' Hleq' Hstep'. eapply bstep_e_deterministic in H11; eauto.
-    inv H11.
+    inv H11. 
     edestruct IHe as [v2'' [c2 [Hstep2 Happrox2]]];
-        [| now eauto | | | eassumption | eassumption | eassumption | ]. 
+        [| now eauto | | | | | eassumption | eassumption | eassumption | ]. 
     + eapply cc_approx_env_P_extend with (v2 := Vconstr tau' t0 v').
       rewrite Setminus_Union_distr,
       Setminus_Empty_set, Union_Empty_set_r. 
@@ -927,6 +1410,9 @@ Proof.
       eapply Setminus_Included. now apply Included_refl.
       rewrite cc_approx_val_eq. constructor; eauto.
       now eapply Forall2_Forall2_asym_included.
+    + eapply vars_in_env_antimon; [| eapply vars_in_env_extend; eassumption ].
+      eapply occurs_free_Econstr_Included. 
+    + intros f Hfin. eauto.
     + eapply Fun_inv_set_In_Scope_l. now eauto.
       eapply Fun_inv_set_In_Scope_r_not_Γ. now eauto.
       intros Heq; subst. now eauto.
@@ -951,10 +1437,14 @@ Proof.
         destruct vcon; try contradiction. inv Happrox2.
         edestruct IHe as [v2 [c2 [Hstep2 Happrox2]]];
           [ eassumption
-          | now intros Hc; eapply Hnin; rewrite bound_var_Ecase_cons; eauto
+          | now intros Hc; eapply Hnin; rewrite bound_var_Ecase_cons; eauto | | 
           | eassumption | eassumption | eassumption | eassumption | eassumption | ].
-        repeat eexists; [| eassumption ].
-        econstructor; eauto. simpl. now rewrite Heq.
+        + eapply vars_in_env_antimon; [|  eassumption ].
+          eapply occurs_free_Ecase_Included. now constructor.
+        + intros f Hfin. eapply Hun.
+          econstructor. eassumption. now constructor. 
+        + repeat eexists; [| eassumption ].
+          econstructor; eauto. simpl. now rewrite Heq.
       - edestruct Hfun as [tau1 [t1 [vs1 [Hget1 Hfun']]]].
         edestruct Hfun' as
             [rho1' [B1 [f1 [rho2' [B2 [f2 [tau2 [t2 [Heq' [Hget2 Happrox2]]]]]]]]]];
@@ -964,12 +1454,16 @@ Proof.
         rewrite cc_approx_val_eq in Happrox2.
         destruct v'; try contradiction. inv Happrox2.
         edestruct IHe as [v2 [c2 [Hstep2 Happrox2]]];
-          [| now intros Hc; eapply Hnin; rewrite bound_var_Ecase_cons; eauto
+          [| now intros Hc; eapply Hnin; rewrite bound_var_Ecase_cons; eauto | |
            | | | eassumption | eassumption | eassumption
            | repeat eexists; [| eassumption ]; econstructor; eauto;
              econstructor; eauto;
              [ rewrite M.gss ; reflexivity | simpl; now rewrite Heq ] ].
         + eapply cc_approx_env_P_not_in_P_r; now eauto.
+        + eapply vars_in_env_antimon; [|  eassumption ].
+          eapply occurs_free_Ecase_Included. now constructor.
+        + intros f Hfin. eapply Hun.
+          econstructor. eassumption. now constructor. 
         + eapply Fun_inv_set_not_In_Funs_r_not_Γ. now eauto.
           intros Heq'; subst. now eauto. eassumption.
         + eapply env_inv_extend_r. intros Hc. subst. now eauto.
@@ -980,12 +1474,16 @@ Proof.
         destruct vcon; try contradiction. inv Happrox2.
         edestruct IHe0 as [v2 [c2' [Hstep2 Happrox2]]];
           [ eassumption
-          | now intros Hc; eapply Hnin; rewrite bound_var_Ecase_cons; eauto
+          | now intros Hc; eapply Hnin; rewrite bound_var_Ecase_cons; eauto | |
           | eassumption | eassumption | now econstructor; eauto
           | eassumption | now econstructor; eauto | ].
-        inv Hstep2. repeat eexists; [| eassumption ].
-        econstructor; eauto. simpl. rewrite Hget' in H5. inv H5.
-        now rewrite Heq. 
+        + eapply vars_in_env_antimon; [| eassumption ].
+          intros x Hin. inv Hin; eauto.
+        + intros f Hfin. eapply Hun. inv Hfin. 
+          econstructor; eauto. constructor 2. eassumption.
+        + inv Hstep2. repeat eexists; [| eassumption ].
+          econstructor; eauto. simpl. rewrite Hget' in H5. inv H5.
+          now rewrite Heq. 
       - edestruct Hfun as [tau1 [t1 [vs1 [Hget1 Hfun']]]].
         edestruct Hfun' as
             [rho1' [B1 [f1 [rho2' [B2 [f2 [tau2 [t2 [Heq' [Hget2 Happrox2]]]]]]]]]];
@@ -996,13 +1494,17 @@ Proof.
         destruct v'; try contradiction. inv Happrox2.
         edestruct IHe0 as [v2 [c2' [Hstep2 Happrox2]]];
           [ eassumption
-          | now intros Hc; eapply Hnin; rewrite bound_var_Ecase_cons; eauto
+          | now intros Hc; eapply Hnin; rewrite bound_var_Ecase_cons; eauto | |
           | eassumption | eassumption | now econstructor; eauto | eassumption
           | now econstructor; eauto | ].
-        inv Hstep2; rewrite Hget in H16; inv H16; rewrite Hnth' in H17; inv H17.
-        inv H18. repeat eexists; [| eassumption ]; econstructor; eauto.
-        econstructor; eauto. simpl.
-        rewrite M.gss in H10. inv H10. now rewrite Heq. }
+        + eapply vars_in_env_antimon; [|  eassumption ].
+          intros x Hin. inv Hin; eauto.
+        + intros f Hfin. eapply Hun. inv Hfin.
+          econstructor; eauto. constructor 2. eassumption.
+        + inv Hstep2; rewrite Hget in H16; inv H16; rewrite Hnth' in H17; inv H17.
+          inv H18. repeat eexists; [| eassumption ]; econstructor; eauto.
+          econstructor; eauto. simpl.
+          rewrite M.gss in H10. inv H10. now rewrite Heq. }
   - (* Case Eproj *)
     inv Hcc.
     intros v1 c1 Hleq Hstep. inv Hstep.
@@ -1015,12 +1517,15 @@ Proof.
     intros v1' c1' Hleq' Hstep'. eapply bstep_e_deterministic in H11; eauto.
     inv H11. edestruct (@Forall2_asym_nthN val) as [v2' [Hnth2 Happ2]]; eauto.
     edestruct IHe as [v2'' [c2 [Hstep2 Happrox2]]];
-        [| now eauto | | | eassumption | eassumption | eassumption | ]. 
+        [| now eauto | | | | | eassumption | eassumption | eassumption | ]. 
     + eapply cc_approx_env_P_extend; [| eassumption ].
       rewrite Setminus_Union_distr,
       Setminus_Empty_set, Union_Empty_set_r. 
       eapply cc_approx_env_P_antimon; [ eassumption |].
       eapply Setminus_Included. now apply Included_refl.      
+    + eapply vars_in_env_antimon; [| eapply vars_in_env_extend; eassumption ].
+      eapply occurs_free_Eproj_Included. 
+    + intros f Hfin. eauto.
     + eapply Fun_inv_set_In_Scope_l. now eauto.
       eapply Fun_inv_set_In_Scope_r_not_Γ. now eauto.
       intros Heq; subst. now eauto.
@@ -1032,69 +1537,157 @@ Proof.
     + repeat eexists; [| eassumption ].
       econstructor; eauto.
   - (* Case Efun -- the hardest one! *) 
-    inv Hcc. 
-    (* edestruct Henv as [tau' [t' [vs' [Hget Hclo]]]].  *)
-    (* eapply closure_conversion_fundefs_correct with *)
-    (* (rho := rho) (rho' := rho') in H3 ; eauto. *)
-    admit.
+    inv Hcc.
+    assert (Ha : exists vs, getlist FVs' rho1 = Some vs).
+    { eapply In_getlist. intros x Hin. eapply HFVs. 
+      rewrite occurs_free_Efun, H1. eauto. }
+    destruct Ha as [vs Hgetlist].
+    intros v1 c1 Hleq Hstep.
+    edestruct project_vars_ctx_to_rho as [rho2' Hto_rho]; eauto.
+    eapply Complement_Disjoint. now apply Included_refl.
+    edestruct project_vars_correct as [Happ [Hfun' [Henv' Hvar]]]; eauto.
+    eapply Complement_Disjoint. now apply Included_refl.
+    edestruct Hvar as [v' [Hget' Happ']]; eauto.
+    eapply ctx_to_rho_cc_approx_exp; eauto.
+    assert (Hsuf :
+              cc_approx_exp k (e, def_funs f2 f2 rho1 rho1)
+                            (C |[ e'0 ]|, def_funs B' B' (M.set Γ' (Vconstr tau t v') rho2')
+                                       (M.set Γ' (Vconstr tau t v') rho2'))).
+    { edestruct make_closures_ctx_to_rho as [rho2'' Htp_rho']; eauto.
+      - eapply closure_conversion_fundefs_correct; eauto.
+        + intros f Hfin. inv Hfin; eauto.
+        + eapply vars_in_env_antimon; [| eassumption ].
+          intros x H. eapply Free_Efun2. eassumption. 
+        + edestruct Hvar as [vs' [Hgetlist' Hall]]; eauto.
+          intros x N v _ _ Hnth Hget. rewrite Hget' in Hgetlist'; inv Hgetlist'.
+          edestruct getlist_nth_get as [v' [Hnth' Hget'']].
+          now apply Hgetlist. eassumption.
+          edestruct (@Forall2_nthN val) as [v'' [Hget''' Hcc'']]. eassumption.
+          eassumption. rewrite Hget in Hget''. inv Hget''. eauto.
+      - intros. now eapply get_def_funs_In_names.
+      - edestruct make_closures_correct with
+          (Scope := Union var (name_in_fundefs f2) Scope)
+          (Γ := Γ)
+          (rho1 := def_funs f2 f2 rho1 rho1)
+          (rho2 := def_funs B' B' (M.set Γ' (Vconstr tau t v') rho2')
+                            (M.set Γ' (Vconstr tau t v') rho2'))
+          as [Hcc'' [Hfun'' Henv'']].
+        + eauto.
+        + eauto.
+        + intros Hc. eapply Hnin. constructor.
+          now eapply name_in_fundefs_bound_var_fundefs.
+        + eauto.
+        + eapply Included_Union_l.
+        + eapply cc_approx_env_P_def_funs_not_In_P_l.
+          eapply Disjoint_Setminus. now apply Included_refl.
+          eapply cc_approx_env_P_def_funs_not_In_P_r.
+          eapply Disjoint_Setminus. rewrite <- Closure_conversion_fundefs_name_in_fundefs.
+          now apply Included_refl. eauto.
+          eapply cc_approx_env_P_not_in_P_r.
+          eapply cc_approx_env_P_antimon. eassumption.
+          rewrite Setminus_Union_distr, Setminus_Empty_set, Union_Empty_set_r.
+          eapply Setminus_Included. now apply Included_refl.
+          intros Hin. inv Hin. eapply H2. inv H; eauto.
+        + eapply Fun_inv_def_funs.
+          * intros Hc. eapply Hnin. constructor.
+            now eapply name_in_fundefs_bound_var_fundefs.
+          * eapply Closure_conversion_fundefs_name_in_fundefs. eassumption.
+          * eapply Fun_inv_set_not_In_Funs_r_not_Γ; [| | eassumption ].
+            intros Hc. eapply H2. eauto.
+            intros Hc. eapply H2. subst. eauto.
+        + eapply env_inv_def_funs.
+          * intros Hc. eapply Hnin. constructor.
+            now eapply name_in_fundefs_bound_var_fundefs.
+          * eapply Closure_conversion_fundefs_name_in_fundefs. eassumption.
+          * eapply  env_inv_extend_r.
+            intros Hc. eapply H2. subst. eauto.
+            eassumption. 
+        + eapply closure_conversion_fundefs_correct; eauto.
+          * intros f Hfin. inv Hfin; eauto.
+          * eapply vars_in_env_antimon; [| eassumption ].
+            intros x H. eapply Free_Efun2. eassumption. 
+          * edestruct Hvar as [vs' [Hgetlist' Hall]]; eauto.
+            intros x N v _ _ Hnth Hget. rewrite Hget' in Hgetlist'; inv Hgetlist'.
+            edestruct getlist_nth_get as [v' [Hnth' Hget'']].
+            now apply Hgetlist. eassumption.
+            edestruct (@Forall2_nthN val) as [v'' [Hget''' Hcc'']]. eassumption.
+            eassumption. rewrite Hget in Hget''. inv Hget''. eauto.
+        + eauto.
+        + eapply ctx_to_rho_cc_approx_exp; eauto.
+          eapply IHe; eauto.
+          * eapply vars_in_env_antimon.
+            eapply Included_trans. now eapply occurs_free_Efun_Included.
+            rewrite Union_sym. now apply Included_refl.
+            apply vars_in_env_def_funs. eassumption.
+          * intros f Hfin; eauto. }
+    intros v1' c1' Hleq' Hstep'. inv Hstep'.
+    edestruct Hsuf as [v2' [c2' [Hstep2' Hcc2']]]; [| eassumption |]; eauto.
+    repeat eexists; eauto. econstructor; eauto.
+    econstructor; eauto.
   - (* Case Eapp *)
     inv Hcc.
     intros v1 c1 Hleq Hstep. inv Hstep.
     + edestruct project_vars_ctx_to_rho as [rho2' Hto_rho]; eauto.
       eapply Complement_Disjoint. now apply Included_refl.      
-      simpl. rewrite H3, H7. reflexivity.
+      simpl. rewrite H4, H8. reflexivity.
       edestruct project_vars_correct as [Happ [Hfun' [Henv' Hvar]]]; eauto.
       eapply Complement_Disjoint. now apply Included_refl.
       edestruct Hvar as [v' [Hget' Happ']]; eauto.
-      simpl. rewrite H3, H7. reflexivity.
+      simpl. rewrite H4, H8. reflexivity.
       simpl in Hget'. destruct (M.get f' rho2') eqn:Hgetf'; try discriminate.
       destruct (getlist ys' rho2') eqn:Hgetlist'; try discriminate. inv Hget'.
-      inv Happ'. rewrite cc_approx_val_eq in H4. destruct v0; try contradiction.
+      inv Happ'. rewrite cc_approx_val_eq in H5. destruct v0; try contradiction.
       eapply ctx_to_rho_cc_approx_exp with (e := Eapp v l); eauto.
       * intros v1' c1' Hleq' Hstep'.
-        inv Hstep'. rewrite H3 in H5. inv H5.
-        rewrite H7 in H12; inv H12.
+        inv Hstep'. rewrite H4 in H6. inv H6.
+        rewrite H8 in H13; inv H13.
         admit. (* the relation needs tweaking *)
-        rewrite H3 in H2. congruence.
+        rewrite H4 in H3. congruence.
       * constructor; eauto.
     + edestruct project_vars_ctx_to_rho as [rho2' Hto_rho]; eauto.
       eapply Complement_Disjoint. now apply Included_refl.      
-      simpl. rewrite H2, H3. reflexivity.
+      simpl. rewrite H3, H4. reflexivity.
       edestruct project_vars_correct as [Happ [Hfun' [Henv' Hvar]]]; eauto.
       eapply Complement_Disjoint. now apply Included_refl.
       edestruct Hvar as [v' [Hget' Happ']]; eauto.
-      simpl. rewrite H2, H3. reflexivity.
+      simpl. rewrite H3, H4. reflexivity.
       simpl in Hget'. destruct (M.get f' rho2') eqn:Hgetf'; try discriminate.
       destruct (getlist ys' rho2') eqn:Hgetlist'; try discriminate. inv Hget'.
-      inv Happ'. rewrite cc_approx_val_eq in H9. destruct v0; try contradiction.
+      inv Happ'. rewrite cc_approx_val_eq in H10. destruct v0; try contradiction.
       eapply ctx_to_rho_cc_approx_exp with (e := Eapp v l); eauto.
       * intros v1' c1' Hleq' Hstep'.
         inv Hstep'.
-        { rewrite H3 in H15. inv H15. 
-          rewrite H2 in H10; inv H10. }
-        { rewrite H3 in H10. inv H10. 
-          rewrite H2 in H5; inv H5.
+        { rewrite H4 in H16. inv H16. 
+          rewrite H3 in H11; inv H11. }
+        { rewrite H4 in H11. inv H11. 
+          rewrite H3 in H6; inv H6.
           destruct l1; try contradiction. destruct v0, l1; try contradiction.
-          destruct v2; try contradiction. simpl in H9.
-          rewrite H13 in H4. inv H4. 
-          rewrite H7 in H15. inv H15. eapply bstep_e_deterministic in H18; eauto. inv H18.
-          assert (Hlen := List_util.Forall2_length _ _ _ H12).
-          edestruct H9 with (vs2 := l0) (j := k - 1)
+          destruct v2; try contradiction.
+          rewrite H14 in H5. inv H5. 
+          rewrite H8 in H16. inv H16. eapply bstep_e_deterministic in H19; eauto. inv H19.
+          assert (Hlen := List_util.Forall2_length _ _ _ H13).
+          edestruct H10 with (vs2 := l0) (j := k - 1)
             as [t2' [Γ' [xs2 [e2 [rho2'' [Hfind [Hset Hyp]]]]]]]; eauto.
           edestruct Hyp as [v2' [c2 [Hstep2 Hcc']]]; try eassumption. omega.
           eapply List_util.Forall2_monotonic; [| eassumption ].
           intros. eapply cc_approx_val_monotonic. eassumption. omega. omega.
           repeat eexists; eauto. econstructor. eassumption. reflexivity.
-          econstructor. rewrite M.gso. eassumption. admit.
+          econstructor. rewrite M.gso. eassumption.
+          intros Hc; subst. eapply project_vars_not_In_free_set. eauto.
+          eapply Complement_Disjoint. now apply Included_refl.
+          constructor. now eapply H2. rewrite FromList_cons. now eauto.
           reflexivity.
           eapply BStep_app_fun. rewrite M.gso. rewrite M.gss. reflexivity.
-          admit. simpl. rewrite M.gss.
-          assert (Ha :
-                    getlist ys'
-                            (M.set env' (Vconstr t4 t5 l2) (M.set f'' (Vfun t3 f v0) rho2')) = Some l0)
-            by admit.
-          rewrite Ha. reflexivity. eassumption.
-          eauto. eassumption. simpl.
+          now eauto. simpl. rewrite M.gss.
+          rewrite getlist_set_neq. rewrite getlist_set_neq.
+          rewrite Hgetlist'. reflexivity. 
+          intros Hin. eapply project_vars_not_In_free_set. eassumption.
+          eapply Complement_Disjoint. now apply Included_refl.
+          constructor. eapply H2. rewrite FromList_cons. now eauto.
+          intros Hin. eapply project_vars_not_In_free_set. eassumption.
+          eapply Complement_Disjoint. now apply Included_refl.
+          constructor. eapply H7. rewrite FromList_cons. now eauto.
+          eassumption. simpl in Hset. eauto. eassumption.
           eapply cc_approx_val_monotonic. eassumption. omega. }
         * econstructor; eauto. 
   - inv Hcc.
@@ -1109,12 +1702,15 @@ Proof.
     inv H11.
     edestruct Prim_axiom as [vs' [Hf' Hcc]]; eauto.
     edestruct IHe as [v2'' [c2 [Hstep2 Happrox2]]];
-        [| now eauto | | | eassumption | eassumption | eassumption | ]. 
+        [| now eauto | | | | | eassumption | eassumption | eassumption | ]. 
     + eapply cc_approx_env_P_extend; [| eassumption ].
       rewrite Setminus_Union_distr,
       Setminus_Empty_set, Union_Empty_set_r. 
       eapply cc_approx_env_P_antimon; [ eassumption |].
       eapply Setminus_Included. now apply Included_refl.
+    + eapply vars_in_env_antimon; [| eapply vars_in_env_extend; eassumption ].
+      eapply occurs_free_Eprim_Included. 
+    + intros f Hfin. eauto.
     + eapply Fun_inv_set_In_Scope_l. now eauto.
       eapply Fun_inv_set_In_Scope_r_not_Γ. now eauto.
       intros Heq; subst. now eauto.
@@ -1125,4 +1721,4 @@ Proof.
       subst. now eauto. now eapply env_inv_extend_Scope.
     + repeat eexists; [| eassumption ].
       econstructor; eauto.
-Abort.
+Admitted.
